verif/trie/functional/trie.v
@@ -5,6 +5,7 @@ Require Import common.
 Require Import DB.lemmas.
 
 Require Import DB.functional.kv.
+Require Import DB.functional.cursored_kv.
 Require Import DB.functional.keyslice.
 Require Import DB.functional.bordernode.
 
@@ -25,31 +26,367 @@ End TrieKey.
 
 Module KeysliceType := Z_as_OT.
 
-Module Trie.
-  Definition key: Type := TrieKey.t.
+(* On going rewrite:
+ * 1. support cursor
+ * 2. add addresses into the data type.
+ *)
 
-  Module SortedListTable := SortedListTable KeysliceType.
+Module Trie (Node: FLATTENABLE_TABLE KeysliceType) <: FLATTENABLE_TABLE TrieKey.
+  Definition key := TrieKey.t.
 
-  Section Parametrized.
+  Module Flattened := SortedListTable TrieKey.
+
+  Section Types.
     Context {value: Type}.
+    (* Notes: reason for removing the [val] from the constructor:
+     *        originally the kvstore contains a cursor for it, therefore there is necessity for another struct,
+     *        it's not the case in final impl, and therefore we directly use the btree as pointer to a trienode *)
     Inductive trie: Type :=
-    | trienode_of: list (keyslice * (list link * option string * link)) -> trie
+    | trienode_of: Node.table val -> (* The btree data *)
+                   Node.Flattened.table (@BorderNode.table link) -> (* abstract data *)
+                   trie
     with
     link: Type :=
     | value_of: value -> link
     | trie_of: trie -> link
     | nil: link.
+    Definition table: Type := trie.
     Hint Constructors trie: trie.
+    (* order of bordernode? *)
+    (* first the prefixes, then the suffix? *)
+    (* Placement of cursor:
+     * For keys that already existed in the store, just place at the place
+     * For keys that are not in the store, place them at the furtherest bordernode entry *)
+    Definition cursor: Type := list (trie * Node.cursor val * option Z).
+    Definition allocator: Type := list val.
+
+    Definition consume (a: allocator) := (hd default a, tl a).
+
+    Definition empty (a: allocator) :=
+      let (empty_table, a) := Node.empty a in
+      (trienode_of empty_table [], a).
 
     Instance inh_link: Inhabitant link := nil.
     Instance dft_link: DefaultValue link := nil.
 
+    Fixpoint flatten_aux (prefix: string) (t: trie) {struct t}: Flattened.table value :=
+      let flatten_link :=
+        fun (prefix: string) (l: link) =>
+          match l with
+          | value_of v => [(prefix, v)]
+          | trie_of t => flatten_aux prefix t
+          | nil => []
+          end
+      in
+        let flatten_prefix_array (prefix: string) (keyslice: KeysliceType.t) :=
+            fix flatten_prefix_array (prefixes: list link) (idx: Z) :=
+            match prefixes with
+            | h :: t =>
+              flatten_link (prefix ++ (reconstruct_keyslice (keyslice, idx))) h ++ flatten_prefix_array t (idx + 1)
+            | [] => []
+            end
+      in
+      let flatten_bordernode :=
+          fun (prefix: string) (kv: KeysliceType.t * @BorderNode.table link) =>
+          let (keyslice, bnode) := kv in
+          match bnode with
+          | (prefixes, Some suffix, l) =>
+            flatten_prefix_array prefix keyslice prefixes 1 ++ flatten_link (prefix ++ suffix) l
+          | (prefixes, None, v) =>
+            flatten_prefix_array prefix keyslice prefixes 1 ++ flatten_link prefix v
+          end
+      in
+      match t with
+      (* the tableform is of no interest here *)
+      | trienode_of _ listform =>
+        flat_map (flatten_bordernode prefix) listform
+      end.
+
+    Definition flatten (t: trie): Flattened.table value := flatten_aux [] t.
+
+    Function make_cursor (k: key) (t: trie) {measure length k}: cursor :=
+      let keyslice := get_keyslice k in
+      match t with
+      | trienode_of tableform listform =>
+        match Node.Flattened.get_value (Node.Flattened.make_cursor (keyslice) listform) listform with
+        | Some bnode =>
+          if (Z_le_dec (Zlength k) keyslice_length) then
+          (* prefix case, which we need only to return the current cursor *)
+            [(t, Node.make_cursor keyslice tableform, Some (Zlength k))]
+          else
+            if BorderNode.is_link bnode then
+              match BorderNode.get_suffix None bnode with
+              | value_of _ => []
+              | nil => []
+              | trie_of t' =>
+                (t, Node.make_cursor keyslice tableform, None) :: make_cursor (get_suffix k) t'
+              end
+            else
+              [(t, Node.make_cursor keyslice tableform, None)]
+        | None =>
+          []
+        end
+      end.
+    Proof.
+      intros.
+      unfold get_suffix.
+      rewrite Nat2Z.inj_lt.
+      rewrite <- ?Zlength_correct.
+      assert (Zlength k > keyslice_length) by (apply Znot_le_gt; assumption).
+      rewrite Zlength_sublist by rep_omega.
+      rep_omega.
+    Defined.
+
+    Fixpoint get_key (c: cursor) (t: trie): option key :=
+      match c with
+      | (_, _, inr (Some _)) :: _ :: _ => (* invalid cursor: suffix portion but not last slice *)
+        None
+      | (_, _, inl _) :: _ :: _ => (* invalid cursor: prefix portion but not last slice *)
+        None
+      | [] => (* invalid cursor: reach the end of cursor slices without ending in either prefix of suffix *)
+        None
+      | [(_, table_cursor, inr (Some suffix))] => (* valid cursor: at the end we reach a suffix portion *)
+        Some suffix
+      | [(t, table_cursor, inl len)] => (* valid cursor: at the end we reach a prefix portion *)
+        let (_, tableform, _) := t in
+        match NodeTable.get_key table_cursor tableform with
+        | Some keyslice => Some (reconstruct_keyslice (keyslice, len))
+        | None => None
+        end
+      | (t, table_cursor, inr None) :: c' => (* recursive part *)
+        let (_, tableform, listform) := t in
+        match NodeTable.get_key table_cursor tableform with
+        | Some keyslice =>
+          match NodeTable.Flattened.get keyslice listform with
+          | Some bnode =>
+            match BorderNode.get_suffix None bnode with
+            | value_of _ => None
+            | nil => None
+            | trie_of t' =>
+              match get_key c' t' with
+              | Some k' => Some ((reconstruct_keyslice (keyslice, keyslice_length)) ++ k')
+              | None => None
+              end
+            end
+          | None => None (* impossible *)
+          end
+        | None => None
+        end
+      end.
+
+    Fixpoint get (c: cursor) (t: trie): option value :=
+      match c with
+      | (_, _, inr (Some _)) :: _ :: _ => (* invalid cursor: suffix portion but not last slice *)
+        None
+      | (_, _, inl _) :: _ :: _ => (* invalid cursor: prefix portion but not last slice *)
+        None
+      | [] => (* invalid cursor: reach the end of cursor slices without ending in either prefix of suffix *)
+        None
+      | [(t, table_cursor, inr (Some suffix))] => (* valid cursor: at the end we reach a suffix portion *)
+        let (_, tableform, listform) := t in
+        match NodeTable.get_key table_cursor tableform with
+        | Some keyslice =>
+          match NodeTable.Flattened.get keyslice listform with
+          | Some bnode =>
+            match BorderNode.get_suffix (Some suffix) bnode with
+            | value_of v => Some v
+            | nil => None
+            | trie_of _ => None
+            end
+          | None => None (* impossible *)
+          end
+        | None => None
+        end
+      | [(t, table_cursor, inl len)] => (* valid cursor: at the end we reach a prefix portion *)
+        let (_, tableform, listform) := t in
+        match NodeTable.get_key table_cursor tableform with
+        | Some keyslice =>
+          match NodeTable.Flattened.get keyslice listform with
+          | Some bnode =>
+            match BorderNode.get_prefix len bnode with
+            | value_of v => Some v
+            | nil => None
+            | trie_of _ => None
+            end
+          | None => None (* impossible *)
+          end
+        | None => None
+        end
+      | (t, table_cursor, inr None) :: c' => (* recursive part *)
+        let (_, tableform, listform) := t in
+        match NodeTable.get_key table_cursor tableform with
+        | Some keyslice =>
+          match NodeTable.Flattened.get keyslice listform with
+          | Some bnode =>
+            match BorderNode.get_suffix None bnode with
+            | value_of _ => None
+            | nil => None
+            | trie_of t' =>
+              match get c' t' with
+              | Some v => Some v
+              | None => None
+              end
+            end
+          | None => None (* impossible *)
+          end
+        | None => None
+        end
+      end.
+
+    (* For now, the definition of put ignore the cursor for simplicity *)
+
+    Definition create_pair_aux_dec {A: Type}: forall k1 k2: list A,
+        {Zlength k1 <= keyslice_length \/ Zlength k2 <= keyslice_length} +
+        {Zlength k1 > keyslice_length /\ Zlength k2 > keyslice_length}.
+    Proof.
+      intros.
+      destruct (Z_le_gt_dec (Zlength k1) keyslice_length);
+        destruct (Z_le_gt_dec (Zlength k2) keyslice_length);
+        match goal with
+        | [H: _ <= _ |- _] => left; omega
+        | _ => right; omega
+        end.
+    Qed.
+
+    Definition consume_addr (l: list val) :=
+      (hd default l, tl l).
+
+
+    Function create_pair (k1 k2: key) (v1 v2: link) (l: list val) {measure length k1} : trie :=
+      let keyslice1 := get_keyslice k1 in
+      let keyslice2 := get_keyslice k2 in
+      if eq_dec keyslice1 keyslice2 then
+        if create_pair_aux_dec k1 k2 then
+          let bnode := BorderNode.put_value k2 v2 (BorderNode.put_value k1 v1 BorderNode.empty) in
+          let (trie_addr, l) := consume_addr l in
+          let (bnode_addr, l) := consume_addr l in
+          trienode_of trie_addr
+                      (NodeTable.put keyslice2 bnode_addr l (NodeTable.first_cursor NodeTable.empty) NodeTable.empty)
+                      (NodeTable.Flattened.put keyslice2 bnode NodeTable.Flattened.empty)
+        else
+          trienode_of (
+              NodeTable.Flattened.put keyslice1 (
+                                    BorderNode.put_suffix None (
+                                                            trie_of (create_pair (get_suffix k1) (get_suffix k2) v1 v2)
+                                                          ) BorderNode.empty
+                                  ) NodeTable.Flattened.empty
+            )
+      else
+        let tmp := NodeTable.Flattened.put keyslice1 (
+                                         BorderNode.put_value k1 v1 BorderNode.empty
+                                       ) NodeTable.Flattened.empty
+        in trienode_of (
+               NodeTable.Flattened.put keyslice2 (
+                                     BorderNode.put_value k2 v2 BorderNode.empty
+                                   ) tmp
+             ).
+    Proof.
+      intros.
+      intros.
+      unfold get_suffix.
+      rewrite Nat2Z.inj_lt.
+      rewrite <- ?Zlength_correct.
+      destruct anonymous0.
+      rewrite Zlength_sublist; repeat first [split | rep_omega | omega].
+    Defined.
+
+    Function put (k: key) (v: value) (t: trie) {measure length k}: trie :=
+      let keyslice := get_keyslice k in
+      match t with
+      | trienode_of trienode =>
+        match NodeTable.Flattened.get keyslice trienode with
+        | Some bordernode =>
+          if Z_le_dec (Zlength k) (keyslice_length) then
+            (* overwrite prefix *)
+            trienode_of (
+                NodeTable.Flattened.put keyslice (
+                                      BorderNode.put_prefix (Zlength k) (value_of v) bordernode
+                                    ) trienode
+              )
+          else
+            if BorderNode.is_link bordernode then
+              match BorderNode.get_suffix None bordernode with
+              | value_of _ => empty
+              | trie_of t' =>
+                (* pass down to next layer *)
+                trienode_of (
+                    NodeTable.Flattened.put keyslice (
+                                          BorderNode.put_suffix (None) (
+                                                                  trie_of (put (get_suffix k) v t')
+                                                                ) bordernode
+                                        ) trienode
+                  )
+              | nil =>
+                (* new suffix *)
+                trienode_of (
+                    NodeTable.Flattened.put keyslice (
+                                          BorderNode.put_suffix (Some (get_suffix k)) (value_of v) BorderNode.empty
+                                        ) NodeTable.Flattened.empty
+                  )
+              end
+            else
+              if BorderNode.test_suffix (Some (get_suffix k)) bordernode then
+                (* overwrite suffix *)
+                trienode_of (
+                    NodeTable.Flattened.put keyslice (
+                                          BorderNode.put_suffix (Some (get_suffix k)) (value_of v) bordernode
+                                        ) trienode
+                  )
+              else
+                (* new layer with two suffix *)
+                match BorderNode.get_suffix_pair bordernode with
+                | (Some k', v') =>
+                  trienode_of (
+                      NodeTable.Flattened.put keyslice (
+                                            BorderNode.put_suffix
+                                              None (
+                                                trie_of (create_pair (get_suffix k) k' (value_of v) v')
+                                              ) bordernode
+                                          ) trienode
+                    )
+                | (None, v') =>
+                  empty
+                end
+        | None =>
+          (* new btree kv pair *)
+          trienode_of (
+              NodeTable.Flattened.put keyslice (
+                                    BorderNode.put_value k (value_of v) BorderNode.empty
+                                  ) trienode
+            )
+        end
+      end.
+    Proof.
+      intros.
+      intros.
+      unfold get_suffix.
+      rewrite Nat2Z.inj_lt.
+      rewrite <- ?Zlength_correct.
+      assert (Zlength k > keyslice_length) by (apply Znot_le_gt; assumption).
+      rewrite Zlength_sublist by rep_omega.
+      rep_omega.
+    Defined.
+
+    Definition next_cursor (c: cursor) (t: trie): cursor. Admitted.
+    Definition prev_cursor (c: cursor) (t: trie): cursor. Admitted.
+    Definition first_cursor (t: trie): cursor. Admitted.
+    Definition last_cursor (t: trie): cursor. Admitted.
+
+    Definition abs_rel (c: cursor) (t: trie): Prop. Admitted.
+    Definition key_rel (k: key) (c: cursor) (t: trie): Prop :=
+      abs_rel c t /\ get_key c t = Some k.
+    Definition eq_cursor (c1 c2: cursor) (t: table) :=
+      abs_rel c1 t /\ abs_rel c2 t /\ get_key c1 t = get_key c2 t.
+
+    Definition cursor_correct (c: cursor): Prop := True.
+
     Inductive trie_invariant: trie -> Prop :=
     | invariant_trienode:
-        forall trienode,
-          SortedListTable.sorted trienode ->
-          Forall (fun binding => bordernode_invariant (snd binding)) trienode ->
-          trie_invariant (trienode_of trienode)
+        forall v btreeform listform,
+          NodeTable.Flattened.sorted listform ->
+          Forall (fun binding => bordernode_invariant (snd binding)) listform ->
+          map fst (NodeTable.flatten btreeform) = map fst listform ->
+          trie_invariant (trienode_of v btreeform listform)
     with
     bordernode_invariant: BorderNode.table -> Prop :=
     | invariant_bordernode:
@@ -87,44 +424,68 @@ Module Trie.
     Hint Constructors trie_invariant: trie.
     Hint Constructors bordernode_invariant: trie.
     Hint Constructors link_invariant: trie.
-    
-    Definition empty: trie := trienode_of [].
 
-    Lemma empty_invariant: trie_invariant empty.
+    Lemma empty_invariant: forall t, trie_invariant empty.
     Proof.
       constructor; auto with sortedtable.
     Qed.
     Hint Resolve empty_invariant: trie.
 
-    (* Fixpoint trie_height (t: trie): nat := *)
-    (*   match t with *)
-    (*   | trienode_of trienode => *)
-    (*     S (fold_right (fun binding => Nat.max (link_height (snd (snd binding)))) 0%nat trienode) *)
-    (*   end *)
-    (* with *)
-    (* link_height (l: link): nat := *)
-    (*   match l with *)
-    (*   | value_of _ => 0 *)
-    (*   | trie_of t' => trie_height t' *)
-    (*   | nil => 0 *)
-    (*   end. *)
+    Definition table_correct (t: table): Prop. Admitted.
+    Section Specs.
+      Variable t: table elt.
+      Variable c c1 c2 c3: cursor elt.
+      Variable k k1 k2 k3: key.
+      Variable e e1 e2: elt.
 
-    (* Lemma max_in_le {A: Type}: forall (f: A -> nat) (l: list A) (e: A), *)
-    (*     In e l -> *)
-    (*     (f e <= fold_right (fun e' => Nat.max (f e')) 0 l)%nat. *)
-    (* Proof. *)
-    (*   intros. *)
-    (*   induction l. *)
-    (*   - inversion H. *)
-    (*   - simpl. *)
-    (*     inversion H; subst; clear H. *)
-    (*     + apply Nat.le_max_l. *)
-    (*     + specialize (IHl H0). *)
-    (*       apply Nat.max_le_iff. *)
-    (*       right. *)
-    (*       assumption. *)
-    (* Qed. *)
+      Axiom abs_correct: abs_rel c t -> cursor_correct c /\ table_correct t.
+      
+      Hypothesis Htable_correct: table_correct t.
+      Axiom make_cusor_binded: abs_rel (make_cursor k t) t.
+      Axiom put_bind:
+        let (new_cursor, new_table) := put c e t in
+        abs_rel new_cursor new_table.
+      Axiom next_cursor_bind: abs_rel c t -> abs_rel (next_cursor c t) t.
+      Axiom prev_cursor_bind: abs_rel c t -> abs_rel (prev_cursor c t) t.
+      Axiom first_cursor_bind: abs_rel (first_cursor t) t.
+      Axiom last_cursor_bind: abs_rel (last_cursor t) t.
+      Axiom get_put_same:
+        key_rel k c1 (snd (put c2 e t)) ->
+        key_rel k c2 t ->
+        get c1 (snd (put c2 e t)) = Some e.
+      Axiom get_put_diff:
+        k1 <> k2 ->
+        key_rel k1 c1 (snd (put c2 e t)) ->
+        key_rel k2 c2 t ->
+        key_rel k1 c3 t ->
+        get c1 (snd (put c2 e t)) = get c3 t.
 
+      Axiom get_last:
+        get (last_cursor t) t = None.
+      Axiom get_empty:
+        abs_rel c t -> empty t -> get c t = None.
+
+      Axiom make_cursor_key:
+        key_rel k (make_cursor k t) t.
+      Axiom next_prev:
+        abs_rel c t -> ~ eq_cursor c (last_cursor t) t -> eq_cursor c (prev_cursor (next_cursor c t) t) t.
+      Axiom prev_next:
+        abs_rel c t -> ~ eq_cursor c (first_cursor t) t -> eq_cursor c (next_cursor (prev_cursor c t) t) t.
+      Axiom next_order:
+        ~ eq_cursor c (last_cursor t) t -> key_rel k1 c t -> key_rel k2 (next_cursor c t) t -> KeyType.lt k1 k2.
+      Axiom prev_order:
+        ~ eq_cursor c (first_cursor t) t -> key_rel k1 c t -> key_rel k2 (prev_cursor c t) t -> KeyType.lt k2 k1.
+      Axiom next_compact:
+        ~ eq_cursor c (last_cursor t) t ->
+        key_rel k1 c t -> key_rel k2 (next_cursor c t) t ->
+        ~ key_rel k3 c t -> KeyType.lt k1 k3 /\ KeyType.lt k3 k2.
+      Axiom prev_compact:
+        ~ eq_cursor c (first_cursor t) t ->
+        key_rel k1 c t -> key_rel k2 (prev_cursor c t) t ->
+        ~ key_rel k3 c t -> KeyType.lt k2 k3 /\ KeyType.lt k3 k1.
+    End Specs.
+  End Types.
+End Trie.
     Function get (k: key) (t: trie) {measure length k}: option value :=
       let keyslice := get_keyslice k in 
       match t with
@@ -155,134 +516,6 @@ Module Trie.
         end
       end.
     Proof.
-      intros.
-      unfold get_suffix.
-      rewrite Nat2Z.inj_lt.
-      rewrite <- ?Zlength_correct.
-      assert (Zlength k > keyslice_length) by (apply Znot_le_gt; assumption).
-      rewrite Zlength_sublist by rep_omega.
-      rep_omega.
-    Defined.
-
-    Definition create_pair_aux_dec {A: Type}: forall k1 k2: list A,
-        {Zlength k1 <= keyslice_length \/ Zlength k2 <= keyslice_length} +
-        {Zlength k1 > keyslice_length /\ Zlength k2 > keyslice_length}.
-    Proof.
-      intros.
-      destruct (Z_le_gt_dec (Zlength k1) keyslice_length);
-        destruct (Z_le_gt_dec (Zlength k2) keyslice_length);
-        match goal with
-        | [H: _ <= _ |- _] => left; omega
-        | _ => right; omega
-        end.
-    Qed.
-
-    Function create_pair (k1 k2: key) (v1 v2: link) {measure length k1} : trie :=
-      let keyslice1 := get_keyslice k1 in
-      let keyslice2 := get_keyslice k2 in
-      if eq_dec keyslice1 keyslice2 then
-        if create_pair_aux_dec k1 k2 then
-          let tmp := BorderNode.put_value k1 v1 BorderNode.empty
-          in trienode_of (
-                 SortedListTable.put keyslice2 (
-                                       BorderNode.put_value k2 v2 tmp
-                                     ) SortedListTable.empty
-               )
-        else
-          trienode_of (
-              SortedListTable.put keyslice1 (
-                                    BorderNode.put_suffix None (
-                                                            trie_of (create_pair (get_suffix k1) (get_suffix k2) v1 v2)
-                                                          ) BorderNode.empty
-                                  ) SortedListTable.empty
-            )
-      else
-        let tmp := SortedListTable.put keyslice1 (
-                                         BorderNode.put_value k1 v1 BorderNode.empty
-                                       ) SortedListTable.empty
-        in trienode_of (
-               SortedListTable.put keyslice2 (
-                                     BorderNode.put_value k2 v2 BorderNode.empty
-                                   ) tmp
-             ).
-    Proof.
-      intros.
-      intros.
-      unfold get_suffix.
-      rewrite Nat2Z.inj_lt.
-      rewrite <- ?Zlength_correct.
-      destruct anonymous0.
-      rewrite Zlength_sublist; repeat first [split | rep_omega | omega].
-    Defined.
-
-    Function put (k: key) (v: value) (t: trie) {measure length k}: trie :=
-      let keyslice := get_keyslice k in
-      match t with
-      | trienode_of trienode =>
-        match SortedListTable.get keyslice trienode with
-        | Some bordernode =>
-          if Z_le_dec (Zlength k) (keyslice_length) then
-            (* overwrite prefix *)
-            trienode_of (
-                SortedListTable.put keyslice (
-                                      BorderNode.put_prefix (Zlength k) (value_of v) bordernode
-                                    ) trienode
-              )
-          else
-            if BorderNode.is_link bordernode then
-              match BorderNode.get_suffix None bordernode with
-              | value_of _ => empty
-              | trie_of t' =>
-                (* pass down to next layer *)
-                trienode_of (
-                    SortedListTable.put keyslice (
-                                          BorderNode.put_suffix (None) (
-                                                                  trie_of (put (get_suffix k) v t')
-                                                                ) bordernode
-                                        ) trienode
-                  )
-              | nil =>
-                (* new suffix *)
-                trienode_of (
-                    SortedListTable.put keyslice (
-                                          BorderNode.put_suffix (Some (get_suffix k)) (value_of v) BorderNode.empty
-                                        ) SortedListTable.empty
-                  )
-              end
-            else
-              if BorderNode.test_suffix (Some (get_suffix k)) bordernode then
-                (* overwrite suffix *)
-                trienode_of (
-                    SortedListTable.put keyslice (
-                                          BorderNode.put_suffix (Some (get_suffix k)) (value_of v) bordernode
-                                        ) trienode
-                  )
-              else
-                (* new layer with two suffix *)
-                match BorderNode.get_suffix_pair bordernode with
-                | (Some k', v') =>
-                  trienode_of (
-                      SortedListTable.put keyslice (
-                                            BorderNode.put_suffix
-                                              None (
-                                                trie_of (create_pair (get_suffix k) k' (value_of v) v')
-                                              ) bordernode
-                                          ) trienode
-                    )
-                | (None, v') =>
-                  empty
-                end
-        | None =>
-          (* new btree kv pair *)
-          trienode_of (
-              SortedListTable.put keyslice (
-                                    BorderNode.put_value k (value_of v) BorderNode.empty
-                                  ) trienode
-            )
-        end
-      end.
-    Proof.
-      intros.
       intros.
       unfold get_suffix.
       rewrite Nat2Z.inj_lt.
@@ -438,7 +671,7 @@ Module Trie.
         destruct t.
         rewrite put_equation.
         remember (get_keyslice k) as keyslice.
-        remember (SortedListTable.get keyslice l) as btree_result.
+        remember (SortedListTable.get keyslice t) as btree_result.
         destruct btree_result; repeat if_tac; try rep_omega.
         - inv H0.
           constructor.
@@ -478,7 +711,7 @@ Module Trie.
         destruct t.
         rewrite put_equation.
         remember (get_keyslice k) as keyslice.
-        remember (SortedListTable.get keyslice l) as btree_result.
+        remember (SortedListTable.get keyslice t) as btree_result.
         destruct btree_result; repeat if_tac.
         - inv H0.
           constructor.
@@ -495,7 +728,7 @@ Module Trie.
             * rep_omega.
             * assumption.
             * auto with trie.
-        - remember (BorderNode.get_suffix None p) as link.
+        - remember (BorderNode.get_suffix None t0) as link.
           destruct link; auto with trie.
           inv H0.
           constructor; [ auto with sortedtable | ].
@@ -547,7 +780,7 @@ Module Trie.
           apply Znot_le_gt in H1.
           omega.
         - inv H0.
-          destruct p as [[? []]]; [ | contradiction].
+          destruct t0 as [[? []]]; [ | contradiction].
           simpl in *.
           assert (get_suffix k <> s) by (intro; apply H3; f_equal; assumption).
           clear H3.
@@ -562,7 +795,7 @@ Module Trie.
           constructor; [ omega | assumption | ].
           split; auto.
           constructor.
-          destruct H9 as [? []]; destruct l1; try contradiction.
+          destruct H9 as [? []]; destruct l0; try contradiction.
           apply create_pair_invariant;
             repeat first [
                      unfold get_suffix; rewrite Zlength_sublist |
@@ -741,13 +974,13 @@ Module Trie.
         destruct s.
         inv H1.
         remember (get_keyslice k) as keyslice.
-        remember (SortedListTable.get keyslice l) as btree_result.
+        remember (SortedListTable.get keyslice t) as btree_result.
         destruct btree_result; repeat if_tac; rewrite get_equation; try rep_omega.
         - rewrite Heqkeyslice.
           rewrite SortedListTable.get_put_same.
           rewrite if_true by auto.
           rewrite BorderNode.get_put_prefix_same; [ reflexivity | | rep_omega].
-          destruct p as [[]].
+          destruct t0 as [[]].
           unfold BorderNode.invariant.
           simpl.
           symmetry in Heqbtree_result.
@@ -770,13 +1003,13 @@ Module Trie.
         destruct s.
         inv H2.
         remember (get_keyslice k) as keyslice.
-        remember (SortedListTable.get keyslice l) as btree_result.
+        remember (SortedListTable.get keyslice t) as btree_result.
         destruct btree_result; repeat if_tac; rewrite get_equation.
         - rewrite Heqkeyslice.
           rewrite SortedListTable.get_put_same.
           rewrite if_true by auto.
           rewrite BorderNode.get_put_prefix_same; [ reflexivity | | rep_omega].
-          destruct p as [[]].
+          destruct t0 as [[]].
           unfold BorderNode.invariant.
           simpl.
           symmetry in Heqbtree_result.
@@ -800,7 +1033,7 @@ Module Trie.
             rewrite if_false by rep_omega.
             rewrite if_true by auto.
             simpl.
-            destruct t.
+            destruct t0.
             destruct H7.
             inv H2.
             apply H with (Zlength (get_suffix k));
@@ -819,11 +1052,11 @@ Module Trie.
         - rewrite Heqkeyslice.
           rewrite SortedListTable.get_put_same.
           rewrite if_false by rep_omega.
-          destruct p as [[]].
+          destruct t0 as [[]].
           simpl.
           rewrite if_true by auto.
           reflexivity.
-        - destruct p as [[]].
+        - destruct t0 as [[]].
           simpl in *.
           destruct o; try contradiction.
           rewrite Heqkeyslice.
@@ -837,7 +1070,7 @@ Module Trie.
           apply H5 in Heqbtree_result.
           simpl in Heqbtree_result.
           inv Heqbtree_result.
-          destruct l1; try (destruct H11 as [ ? []]; contradiction).
+          destruct l0; try (destruct H11 as [ ? []]; contradiction).
           rewrite get_create_pair_same1.
           + reflexivity.
           + unfold get_suffix.
